\documentclass[a4paper,11pt]{article}
\usepackage[T1]{fontenc}
\usepackage[utf8]{inputenc}
\newcommand\oto{\leftrightarrow}\usepackage{amssymb}
\begin{document}

\noindent Dobre przykłady:

\begin{itemize}
\item $((((p\to q)\to p)\to p)\to q)\to q$;
\item $((((p\to q)\to r)\to(p\to r)\to r)\to q)\to q$;
\item $(p\to q)\oto(((p\to q)\to p)\to q)$;
\item $(p\to q\to r)\to((p\to r)\to s)\to ((q\to r)\to s)\to (s\to r)\to r$;
\item $((((p\to q)\to r)\to (p\to r)\to r)\to q)\to q$;
\item $((p\to q)\to r)\to s\to (q\to r\to t)\to q\to t$.
\end{itemize}

\noindent  Złe przykłady:

\begin{itemize}
\item $(p\to q\to r)\to((p\to r)\to s)\to ((q\to r)\to s)\to s$;
\item $((p\to q)\to r)\to((r\to p)\to r)\to r$;
\item $((p\to q)\to r)\to (p\to r)\to r$;
\item $((p\to q)\to a)\to ((q\to p)\to a)\to a$.
\end{itemize}
\end{document}
